Bachmair_Ganzinger/FO_Resolution_Prover.thy
@@ -115,7 +115,7 @@ qed
 lemma ord_resolve_raw_sound:
   assumes
     res_e: "ord_resolve_raw CC D E" and
-    cc_d_true: "\<And>\<sigma>. is_ground_subst \<sigma> \<Longrightarrow> I \<Turnstile>m (CC + {#D#}) \<cdot>cc \<sigma>" and
+    cc_d_true: "\<And>\<sigma>. is_ground_subst \<sigma> \<Longrightarrow> I \<Turnstile>m (CC + {#D#}) \<cdot>cm \<sigma>" and
     ground_subst_\<sigma>: "is_ground_subst \<sigma>"
   shows "I \<Turnstile> E \<cdot> \<sigma>"
 using res_e proof (cases rule: ord_resolve_raw.cases)
@@ -130,7 +130,7 @@ using res_e proof (cases rule: ord_resolve_raw.cases)
 
   have "is_ground_subst (\<tau> \<odot> \<sigma>)"
     using ground_subst_\<sigma> by (rule is_ground_comp_subst)
-  hence cc_true: "I \<Turnstile>m CC \<cdot>cc \<tau> \<cdot>cc \<sigma>" and d_true: "I \<Turnstile> D \<cdot> \<tau> \<cdot> \<sigma>"
+  hence cc_true: "I \<Turnstile>m CC \<cdot>cm \<tau> \<cdot>cm \<sigma>" and d_true: "I \<Turnstile> D \<cdot> \<tau> \<cdot> \<sigma>"
     using cc_d_true[of "\<tau> \<odot> \<sigma>"] by auto
 
   show ?thesis
@@ -156,10 +156,10 @@ using res_e proof (cases rule: ord_resolve_raw.cases)
       using aaa cabb by force
     { fix B
       assume "B \<in># BB"
-      moreover have "is_unifier_set \<tau> (set_mset AAA)"
-        using \<tau> by (auto simp: aaa intro: is_unifier_set_mgu)
+      moreover have "is_unifiers \<tau> (set_mset AAA)"
+        using \<tau> by (auto simp: aaa intro: is_unifiers_mgu)
       ultimately have "B \<cdot>a \<tau> = A \<cdot>a \<tau>"
-        using a_bb_in_aaa by (intro is_unifier_set_subst_atm_eqI[of "insert A (set_mset BB)"]) auto
+        using a_bb_in_aaa by (intro is_unifiers_subst_atm_eqI[of "insert A (set_mset BB)"]) auto
     }
     hence "\<not> I \<Turnstile> poss BB \<cdot> \<tau> \<cdot> \<sigma>"
       using a_false by (auto simp: true_cls_def)
@@ -175,7 +175,7 @@ qed
 lemma ord_resolve_sound:
   assumes
     res_e: "ord_resolve CC D E" and
-    cc_d_true: "\<And>\<sigma>. is_ground_subst \<sigma> \<Longrightarrow> I \<Turnstile>m (CC + {#D#}) \<cdot>cc \<sigma>" and
+    cc_d_true: "\<And>\<sigma>. is_ground_subst \<sigma> \<Longrightarrow> I \<Turnstile>m (CC + {#D#}) \<cdot>cm \<sigma>" and
     ground_subst_\<sigma>: "is_ground_subst \<sigma>"
   shows "I \<Turnstile> E \<cdot> \<sigma>"
 using res_e proof (cases rule: ord_resolve.cases)
@@ -191,7 +191,7 @@ using res_e proof (cases rule: ord_resolve.cases)
     assume "is_ground_subst \<sigma>"
     hence "is_ground_subst (\<rho> \<odot> \<sigma>)" "\<forall>\<rho>. (\<exists>C. (C, \<rho>) \<in># CCP) \<longrightarrow> is_ground_subst (\<rho> \<odot> \<sigma>)"
       unfolding p by simp_all
-    with cc_d_true have "I \<Turnstile>m (CC\<rho> + {#D \<cdot> \<rho>#}) \<cdot>cc \<sigma>"
+    with cc_d_true have "I \<Turnstile>m (CC\<rho> + {#D \<cdot> \<rho>#}) \<cdot>cm \<sigma>"
       unfolding cc\<rho> cc p
       by (auto simp: subst_cls_comp_subst[symmetric] simp del: subst_cls_comp_subst)
   }
@@ -294,7 +294,7 @@ lemma ord_resolve_lifting:
   obtains \<sigma> CC' D' E' where
     "is_ground_subst \<sigma>"
     "ord_resolve_raw S CC' D' E'"
-    "CC = CC' \<cdot>cc \<sigma>" "D = D' \<cdot> \<sigma>" "E = E' \<cdot> \<sigma>"
+    "CC = CC' \<cdot>cm \<sigma>" "D = D' \<cdot> \<sigma>" "E = E' \<cdot> \<sigma>"
     "{D', E'} \<union> set_mset CC' \<subseteq> M"
 using resolve proof (atomize_elim, cases rule: ord_resolve_raw.cases)
   case (ord_resolve_raw Cf' ZZ AA AAA D' \<sigma>)
@@ -341,7 +341,7 @@ using resolve proof (atomize_elim, cases rule: ord_resolve_raw.cases)
     using pick by auto
 
   obtain \<rho>D \<rho>s where \<rho>s: "length \<rho>s = length Cs" "is_renaming \<rho>D" "\<forall>\<rho> \<in> set \<rho>s. is_renaming \<rho>"
-    "var_disjoint ((Dp \<cdot> \<rho>D) # (Cs \<cdot>cls \<rho>s))"
+    "var_disjoint ((Dp \<cdot> \<rho>D) # (Cs \<cdot>\<cdot>cl \<rho>s))"
     using make_var_disjoint[of "Dp # Cs"] by (auto simp: length_Suc_conv)
 
   from \<rho>s(2,3) obtain \<rho>D' \<rho>'s where "length \<rho>'s = length \<rho>s"
@@ -351,32 +351,32 @@ using resolve proof (atomize_elim, cases rule: ord_resolve_raw.cases)
 
   note lengths = \<open>length \<rho>'s = length \<rho>s\<close> \<rho>s(1) trans[OF \<open>length Cs = ?n\<close> sym[OF \<open>length \<sigma>s = ?n\<close>]]
 
-  then have "Cs \<cdot>cls \<rho>s \<cdot>cls \<rho>'s = Cs" "Dp \<cdot> \<rho>D \<cdot> \<rho>D' = Dp"
+  then have "Cs \<cdot>\<cdot>cl \<rho>s \<cdot>\<cdot>cl \<rho>'s = Cs" "Dp \<cdot> \<rho>D \<cdot> \<rho>D' = Dp"
     unfolding subst_cls_comp_subst[symmetric] subst_cls_lists_comp_substs[symmetric] inv by auto
 
   with lengths var_disjoint_ground[OF \<rho>s(4), of "(\<rho>D' \<odot> \<sigma>D) # (\<rho>'s \<odot>s \<sigma>s)"] ground_\<sigma>D ground_\<sigma>s
-    obtain \<tau> where \<tau>: "is_ground_subst \<tau>" "Dp \<cdot> \<sigma>D = Dp \<cdot> \<rho>D \<cdot> \<tau>" "Cs \<cdot>cls \<sigma>s = Cs \<cdot>cls \<rho>s \<cdot>cl \<tau>"
+    obtain \<tau> where \<tau>: "is_ground_subst \<tau>" "Dp \<cdot> \<sigma>D = Dp \<cdot> \<rho>D \<cdot> \<tau>" "Cs \<cdot>\<cdot>cl \<sigma>s = Cs \<cdot>\<cdot>cl \<rho>s \<cdot>cl \<tau>"
     by auto
 
-  moreover from pick have "?Cs = Cs \<cdot>cls \<sigma>s"
+  moreover from pick have "?Cs = Cs \<cdot>\<cdot>cl \<sigma>s"
     unfolding subst_cls_lists_def Cs_def \<sigma>s_def
     by (auto simp only: set_map length_map length_zip nth_map nth_zip nth_mem list_eq_iff_nth_eq
       set_sorted_list_of_multiset[symmetric])
 
-  then have "mset ?Cs = mset (Cs \<cdot>cls \<sigma>s)"
+  then have "mset ?Cs = mset (Cs \<cdot>\<cdot>cl \<sigma>s)"
     by simp
 
-  ultimately have "D =  Dp \<cdot> \<rho>D \<cdot> \<tau>" "CC = mset (Cs \<cdot>cls \<rho>s) \<cdot>cc \<tau>"
+  ultimately have "D =  Dp \<cdot> \<rho>D \<cdot> \<tau>" "CC = mset (Cs \<cdot>\<cdot>cl \<rho>s) \<cdot>cm \<tau>"
     using pickD by (simp_all add: subst_cls_list_def subst_cls_mset_def mset_map)
 
   def CC' \<equiv> "mset Cs"
   def P \<equiv> "mset \<rho>s"
   def CC'P \<equiv> "mset (zip Cs \<rho>s)"
-  def CC'\<rho> \<equiv> "mset (Cs \<cdot>cls \<rho>s)"
+  def CC'\<rho> \<equiv> "mset (Cs \<cdot>\<cdot>cl \<rho>s)"
   def ZZ\<rho> \<equiv> "ZZ"
 
   show "\<exists>\<sigma> CC' D' E'. is_ground_subst \<sigma> \<and> ord_resolve_raw S CC' D' E' \<and>
-    CC = CC' \<cdot>cc \<sigma> \<and> D = D' \<cdot> \<sigma> \<and> E = E' \<cdot> \<sigma> \<and> {D', E'} \<union> set_mset CC' \<subseteq> M"
+    CC = CC' \<cdot>cm \<sigma> \<and> D = D' \<cdot> \<sigma> \<and> E = E' \<cdot> \<sigma> \<and> {D', E'} \<union> set_mset CC' \<subseteq> M"
   proof (intro exI conjI)
     show "is_ground_subst \<tau>" by (metis \<tau>(1))
     show "ord_resolve_raw S CC'\<rho> (Dp \<cdot> \<rho>D) ((cf + d) \<cdot> x)"
@@ -384,8 +384,8 @@ using resolve proof (atomize_elim, cases rule: ord_resolve_raw.cases)
       apply (simp_all add: selection_renaming_invariant[OF \<rho>s(2)])
       sorry
 
-    show "CC = CC'\<rho> \<cdot>cc \<tau>"
-      unfolding CC'_def CC'\<rho>_def \<open>CC = mset (Cs \<cdot>cls \<rho>s) \<cdot>cc \<tau>\<close> ..
+    show "CC = CC'\<rho> \<cdot>cm \<tau>"
+      unfolding CC'_def CC'\<rho>_def \<open>CC = mset (Cs \<cdot>\<cdot>cl \<rho>s) \<cdot>cm \<tau>\<close> ..
     show "D = Dp \<cdot> \<rho>D \<cdot> \<tau>"
       unfolding \<open>D =  Dp \<cdot> \<rho>D \<cdot> \<tau>\<close> ..
     show "E = (cf + d) \<cdot> x \<cdot> \<tau>"
